Ntt done

proof/spec/Kyber.ec
@@ -442,12 +442,12 @@ op br(i : int) = BitEncoding.BS2Int.bs2int (BitEncoding.BS2Int.int2bs 7 i).
 op ntt(p : poly) = Array256.init (fun i => 
    if i %% 2  = 0 
    then let ii = i %/ 2     in BAdd.bigi predT (fun j => p.[2*j]   * ZqRing.exp zroot ((2 * br ii + 1) * j)) 0 128
-   else let ii = (i-1) %/ 2 in BAdd.bigi predT (fun j => p.[2*j+1] * ZqRing.exp zroot ((2 * br ii + 1) * j)) 0 128).
+   else let ii = (i-1) %/ 2 in BAdd.bigi predT (fun j => p.[2*j+1] * ZqRing.exp zroot ((2 * br ii + 1) * j)) 0 128) axiomatized by nttE.
 
 op invntt(p : poly) = Array256.init (fun i => 
    if i %% 2  = 0 
    then let ii = i %/ 2     in BAdd.bigi predT (fun j => (inv (inFq 128)) * p.[2*j] * ZqRing.exp zroot (-((2 * br ii + 1) * j))) 0 128
-   else let ii = (i-1) %/ 2 in BAdd.bigi predT (fun j => (inv (inFq 128)) * p.[2*j+1] * ZqRing.exp zroot (-((2 * br ii + 1) * j))) 0 128).
+   else let ii = (i-1) %/ 2 in BAdd.bigi predT (fun j => (inv (inFq 128)) * p.[2*j+1] * ZqRing.exp zroot (-((2 * br ii + 1) * j))) 0 128) axiomatized by invnttE.
 
 (* This is multiplication of two degree-1 polynomials in Fq
     modulo X^2 - zroot.
